src/vector.v
@@ -379,7 +379,7 @@ Lemma wp_segment_iteri v xs f :
   ∀Int _i i ,
   ∀Int _k k ,
   valid_seg i k xs →
-  ITER_UP i k
+  ITER_INT_UP i k
     (λ _j j s Q, ∀ x, x = xs !!! j → wp (f _j x s) Q)
     (λ s Q, wp (segment_iteri v _i _k s f) Q).
 Proof.
@@ -396,7 +396,7 @@ Qed.
 
 Lemma wp_iteri v xs f :
   isVector v xs →
-  ITER_UP
+  ITER_INT_UP
     0 (len xs)
     (λ _j j s Q, ∀ x, x = xs !!! j → wp (f _j x s) Q)
     (λ s Q, wp (iteri v s f) Q).
